theories/Equiv/SimLockStep.v
@@ -1,0 +1,98 @@
+Require Import Util Option AllInRel Get.
+Require Export paco2 SmallStepRelations StateType Sim.
+
+Set Implicit Arguments.
+Unset Printing Records.
+
+Inductive sim_gen_lock
+          {S} `{StateType S} {S'} `{StateType S'} (r: S -> S' -> Prop)  : S -> S' -> Prop :=
+  | SimLockSilent (σ1 σ1':S) (σ2 σ2':S') : (* result σ1 = result σ2 -> *)
+      step σ1 EvtTau σ1'
+      -> step σ2 EvtTau σ2'
+      -> r σ1' σ2'
+      -> sim_gen_lock r σ1 σ2
+  | SimLockExtern (σ1:S) (σ2:S') : (* result σ1 = result σ2 -> *)
+      activated σ1
+      -> activated σ2
+      -> (forall evt σ1', step σ1 evt σ1' -> exists σ2', step σ2 evt σ2' /\ r σ1' σ2')
+      -> (forall evt σ2', step σ2 evt σ2' -> exists σ1', step σ1 evt σ1' /\ r σ1' σ2')
+      -> sim_gen_lock r σ1 σ2
+  | SimLockTerm (σ1:S) (σ2:S')
+    : result σ1 = result σ2
+      -> normal2 step σ1
+      -> normal2 step σ2
+      -> sim_gen_lock r σ1 σ2.
+
+Arguments sim_gen_lock [S] {H} [S'] {H0} r _ _.
+
+Hint Constructors sim_gen_lock.
+
+Definition sim_bot {S} `{StateType S} {S'} `{StateType S'} (σ1:S) (σ2:S')
+  := paco2 (@sim_gen_lock S _ S' _) bot2 σ1 σ2.
+
+Hint Unfold sim_bot.
+
+Definition sim_lock {S} `{StateType S} {S'} `{StateType S'} r (σ1:S) (σ2:S')
+  := paco2 (@sim_gen_lock S _ S' _) r σ1 σ2.
+Hint Unfold sim_lock.
+
+Lemma sim_gen_lock_mon {S} `{StateType S} {S'} `{StateType S'}
+: monotone2 (@sim_gen_lock S _ S' _).
+Proof.
+  hnf; intros. inv IN; eauto using @sim_gen_lock.
+  - econstructor 2; eauto; intros.
+    edestruct H3; eauto; dcr. eexists; eauto.
+    edestruct H4; eauto; dcr. eexists; eauto.
+Qed.
+
+Arguments sim_gen_lock_mon [S] {H} [S'] {H0} [x0] [x1] r r' IN LE.
+
+Hint Resolve sim_gen_lock_mon : paco.
+
+Lemma sim_mon S `{StateType S} S' `{StateType S'}
+      (r r':rel2 S (fun (_ : S) => S'))
+  : (forall (x1:S) (x2 : S'), r x1 x2 -> r' x1 x2)
+    -> forall (x:S) (y : S'), sim_lock r x y -> sim_lock r' x y.
+Proof.
+  intros. eapply paco2_mon; eauto.
+Qed.
+
+Hint Resolve sim_mon.
+
+Lemma sim_bisim {S} `{StateType S} {S'} `{StateType S'} (σ:S) (σ':S') t
+      : sim_lock bot2 σ σ' -> sim bot3 t σ σ'.
+Proof.
+  revert σ σ'. pcofix CIH.
+  intros. pinversion H2; subst.
+  - pfold. eapply SimSilent; eauto 20 using plus2O.
+  - pfold. eapply SimExtern; intros; eauto using star2_refl.
+    + edestruct H4; eauto; dcr; pclearbot; eauto 20.
+    + edestruct H5; eauto; dcr; pclearbot; eauto 20.
+  - pfold. eapply SimTerm; eauto using star2_refl.
+Qed.
+
+(** ** Reflexivity, Symmetry *)
+
+Lemma sim_lock_refl {S} `{StateType S} (σ:S) r
+      : sim_lock r σ σ.
+Proof.
+  revert σ.
+  pcofix CIH.
+  intros. destruct (step_dec σ) as [[[] []]|].
+  - pfold. eapply SimLockExtern; intros; eauto using star2_refl; eexists; eauto.
+  - pfold. eapply SimLockSilent; eauto using plus2O.
+  - pfold. eapply SimLockTerm; eauto using star2_refl.
+Qed.
+
+
+Lemma bisim_sym {S} `{StateType S} {S'} `{StateType S'} (σ:S) (σ':S')
+  : sim_lock bot2 σ σ' -> sim_lock bot2 σ' σ.
+Proof.
+  revert σ σ'. pcofix CIH.
+  intros. pinversion H2; subst.
+  - pfold. eapply SimLockSilent; eauto using plus2O.
+  - pfold. eapply SimLockExtern; intros; eauto using star2_refl.
+    + edestruct H5; eauto; dcr; pclearbot; eauto 20.
+    + edestruct H4; eauto; dcr; pclearbot; eauto 20.
+  - pfold. eapply SimLockTerm; eauto using star2_refl.
+Qed.
