theories/Equiv/Tower2.v
@@ -1,0 +1,134 @@
+Require Import Util Option AllInRel Get Setoid.
+Require Export paco2.
+Require Import Coq.Logic.FunctionalExtensionality ClassicalFacts.
+
+Axiom propositional_extensionality : prop_extensionality.
+
+Notation "p =2= q" :=
+  (forall x0 x1, p x0 x1 <-> (q x0 x1:Prop))
+    (at level 50, no associativity).
+
+
+Lemma pred2_extensionality A B (R R' : A -> B -> Prop)
+  : R =2= R' -> R = R'.
+Proof.
+  intros.
+  do 2 (eapply functional_extensionality; intros).
+  eapply propositional_extensionality. eauto.
+Qed.
+
+Set Implicit Arguments.
+
+Section Tower2.
+  Variables A B : Type.
+  Variable f : (A -> B -> Prop) -> (A -> B -> Prop).
+
+  Definition inf2 I (F: I -> A -> B -> Prop) : A -> B -> Prop :=
+    fun a b => forall i:I, F i a b.
+
+  Inductive T2 : (A -> B -> Prop) -> Prop :=
+  | T2_step R : T2 R -> T2 (f R)
+  | T2_lim I (F : I -> A -> B -> Prop)
+    : (forall i, T2 (F i)) -> T2 (inf2 F).
+
+  Definition companion2 (R : A -> B -> Prop) : A -> B -> Prop :=
+    fun a b => forall S, T2 S -> R <2= S -> S a b.
+
+  Notation "'㚘'" := companion2 (at level 0).
+
+  Lemma T_companion2 x : T2 (companion2 x).
+    repeat (eapply T2_lim; intros).
+    eauto.
+  Qed.
+
+  Lemma companion2_monotone : monotone2 companion2.
+    hnf; intros. hnf; intros.
+    eapply IN; eauto.
+  Qed.
+
+  Lemma companion2_inc R : R <2= companion2 R.
+    intros; hnf; eauto.
+  Qed.
+
+  Lemma companion2_idem x : companion2 (companion2 x) = companion2 x.
+    eapply pred2_extensionality; split.
+    - intros H; eapply H; eauto using T_companion2.
+    - eapply companion2_inc.
+  Qed.
+
+
+  Lemma companion2_img x : T2 x -> companion2 x = x.
+    intros. eapply pred2_extensionality.
+    split; intros; eauto using companion2_inc.
+    - eapply H0; eauto.
+  Qed.
+
+  Definition inf2_closed (P: (A -> B -> Prop) -> Prop) :=
+    forall I (F : I -> A -> B -> Prop),
+      (forall i, P (F i)) -> P (inf2 F).
+
+
+  Theorem tower_ind2 P
+    : inf2_closed P ->
+      (forall x, P (companion2 x) -> P (f (companion2 x))) ->
+      forall x, P (companion2 x).
+  Proof.
+    intros.
+    do 3 (eapply H; intros).
+    clear x i1.
+    induction i0; eauto.
+    rewrite <- (companion2_img i0).
+    eapply H0. rewrite companion2_img; eauto.
+  Qed.
+
+  Lemma companion2_fold R
+    : monotone2 f -> f (companion2 R) <2= companion2 R.
+  Proof.
+    intro.
+    eapply tower_ind2.
+    - hnf; intros. hnf; intros. eauto.
+    - intros. eapply H; eauto.
+  Qed.
+
+  Lemma companion2_unfold
+    : companion2 bot2 <2= f (companion2 bot2).
+  Proof.
+    intros. eapply PR; intros.
+    - econstructor 1. eapply T_companion2.
+    - isabsurd.
+  Qed.
+
+  Section UptoLemma2.
+    Variable g : (A -> B -> Prop) -> (A -> B -> Prop).
+    Hypothesis gP : monotone2 g.
+
+    Lemma upto2 :
+      (forall x, g (companion2 x) <2= companion2 x -> g (f (companion2 x)) <2= f (companion2 x)) ->
+      (forall x, g (companion2 x) <2= companion2 x).
+    Proof.
+      intros H1 H2.
+      eapply tower_ind2.
+      - intros; hnf; intros; eauto.
+        hnf; eauto.
+      - intros; eauto.
+    Qed.
+
+    Lemma upto_below2 :
+      (forall x, g (companion2 x) <2= companion2 x) -> g <3= companion2.
+    Proof.
+      intros H1 r; intros.
+      eapply H1. eapply gP; eauto.
+      eapply companion2_inc.
+    Qed.
+
+    Lemma upto_char2 :
+      monotone2 f ->
+      g <3= companion2 ->
+      forall x, g (companion2 x) <2= companion2 x -> g (f (companion2 x)) <2= f (companion2 x).
+    Proof.
+      intros gM H1 r H2; intros.
+      eapply H1; eauto.
+      econstructor 1. eapply T_companion2.
+    Qed.
+  End UptoLemma2.
+End Tower2.
