theories/Equiv/Tower3.v
@@ -1,0 +1,135 @@
+Require Import Util Option AllInRel Get Setoid.
+Require Export paco3.
+Require Import Coq.Logic.FunctionalExtensionality ClassicalFacts.
+
+Axiom propositional_extensionality : prop_extensionality.
+
+Notation "p =3= q" :=
+  (forall x0 x1 x2, p x0 x1 x2 <-> (q x0 x1 x2:Prop))
+    (at level 50, no associativity).
+
+Definition R3Eq A B C (R R' : A -> B -> C -> Prop) :=
+  R =3= R'.
+
+Lemma pred3_extensionality A B C (R R' : A -> B -> C -> Prop)
+  : R =3= R' -> R = R'.
+Proof.
+  intros.
+  do 3 (eapply functional_extensionality; intros).
+  eapply propositional_extensionality. eauto.
+Qed.
+
+Set Implicit Arguments.
+
+Section Tower3.
+  Variables A B C : Type.
+  Variable f : (A -> B -> C -> Prop) -> (A -> B -> C -> Prop).
+
+  Definition inf3 I (F: I -> A -> B -> C -> Prop) : A -> B -> C -> Prop :=
+    fun a b c => forall i:I, F i a b c.
+
+  Inductive T3 : (A -> B -> C -> Prop) -> Prop :=
+  | T3_step R : T3 R -> T3 (f R)
+  | T3_lim I (F : I -> A -> B -> C -> Prop)
+    : (forall i, T3 (F i)) -> T3 (inf3 F).
+
+  Definition companion3 (R : A -> B -> C -> Prop) : A -> B -> C -> Prop :=
+    fun a b c => forall S, T3 S -> R <3= S -> S a b c.
+
+  Notation "'㚘'" := companion3 (at level 0).
+
+  Lemma T_companion3 x : T3 (companion3 x).
+    repeat (eapply T3_lim; intros).
+    eauto.
+  Qed.
+
+  Lemma companion3_monotone : monotone3 companion3.
+    hnf; intros. hnf; intros.
+    eapply IN; eauto.
+  Qed.
+
+  Lemma companion3_inc R : R <3= companion3 R.
+    intros; hnf; eauto.
+  Qed.
+
+  Lemma companion3_idem x : companion3 (companion3 x) = companion3 x.
+    eapply pred3_extensionality. split.
+    - intros H; eapply H; eauto using T_companion3.
+    - eapply companion3_inc.
+  Qed.
+
+  Lemma companion3_img x : T3 x -> companion3 x = x.
+    intros; eapply pred3_extensionality.
+    split; intros; eauto using companion3_inc.
+    eapply H0; eauto.
+  Qed.
+
+  Definition inf3_closed (P: (A -> B -> C -> Prop) -> Prop) :=
+    forall I (F : I -> A -> B -> C -> Prop),
+      (forall i, P (F i)) -> P (inf3 F).
+
+
+  Theorem tower_ind3 P
+    : inf3_closed P ->
+      (forall x, P (companion3 x) -> P (f (companion3 x))) ->
+      forall x, P (companion3 x).
+  Proof.
+    intros.
+    do 3 (eapply H; intros).
+    clear x i1.
+    induction i0; eauto.
+    rewrite <- (companion3_img i0).
+    eapply H0. rewrite companion3_img; eauto.
+  Qed.
+
+  Lemma companion3_fold R
+    : monotone3 f -> f (companion3 R) <3= companion3 R.
+  Proof.
+    intro.
+    eapply tower_ind3.
+    - hnf; intros. hnf; intros. eauto.
+    - intros. eapply H; eauto.
+  Qed.
+
+  Lemma companion3_unfold
+    : companion3 bot3 <3= f (companion3 bot3).
+  Proof.
+    intros. eapply PR; intros.
+    - econstructor 1. eapply T_companion3.
+    - isabsurd.
+  Qed.
+
+  Section UptoLemma3.
+    Variable g : (A -> B -> C -> Prop) -> (A -> B -> C -> Prop).
+    Hypothesis gP : monotone3 g.
+
+    Lemma upto3 :
+      (forall x, g (companion3 x) <3= companion3 x -> g (f (companion3 x)) <3= f (companion3 x)) ->
+      (forall x, g (companion3 x) <3= companion3 x).
+    Proof.
+      intros H1 H2.
+      eapply tower_ind3.
+      - intros; hnf; intros; eauto.
+        hnf; eauto.
+      - intros; eauto.
+    Qed.
+
+    Lemma upto_below3 :
+      (forall x, g (companion3 x) <3= companion3 x) -> g <4= companion3.
+    Proof.
+      intros H1 r; intros.
+      eapply H1. eapply gP; eauto.
+      eapply companion3_inc.
+    Qed.
+
+    Lemma upto_char3 :
+      monotone3 f ->
+      g <4= companion3 ->
+      forall x, g (companion3 x) <3= companion3 x -> g (f (companion3 x)) <3= f (companion3 x).
+    Proof.
+      intros gM H1 r H2; intros.
+      eapply H1; eauto.
+      econstructor 1. eapply T_companion3.
+    Qed.
+  End UptoLemma3.
+End Tower3.
